# Scale-factor-evolution

$\textbf{I - Friedmann's equations}$

In this paper, I won't do the derivation from the Einstein field equations $R_{\mu \nu} - \frac{1}{2} R g_{\mu \nu} + \Lambda g_{\mu \nu} = \frac{8 \pi G}{c^4} T_{\mu \nu}$ to the Friedmann's equations :

$$(1) ~~~~~~~~ \frac{\dot{a}^2}{a^2} = \frac{8 \pi G}{3} \rho - \frac{k}{a^2} + \frac{\Lambda}{3}$$
$$(2) ~~~~~~~~ \frac{\ddot{a}}{a} = - \frac{4 \pi G}{3} (\rho + 3P) + \frac{\Lambda}{3}$$

but we also can specify the law of continuity : $\dot{\rho} = -3 \frac{\dot{a}}{a}(\rho + P) ~~~~~~ (3)$

So from these equations, we're going to compute the numerical solution from a differential equation we're going to derivate.

We also can consider others parameters such as the Hubble constant : $H_0 = H(0) = \frac{\dot{a}(0)}{a(0)}$,
the deceleration parameter $q_0 = q(0) = \big( \frac{\ddot{a}a}{\dot{a}^2} \big )_0$

and the critical density $\rho_c(0) = \rho_{c,0} = \frac{3 H_0^2}{8 \pi G}$

$\textbf{II - Content components of the Universe}$

For a Universe mainly constitutes of a certain content, the evolution of the scale factor will be given by their state equations.

- for the matter : $\Omega_0^M = \frac{\rho_M(0)}{\rho_{0,c} \to \rho_M(t) \propto a(t)^{-3}$
- for the radiation : $\Omega_0^R = \frac{\rho_R(0)}{\rho_{0,c} \to \rho_R(t) \propto a(t)^{-4}$
- for the dark energy : $\Omega_0^{\Lambda} = \frac{\rho_{\Lambda}(0)}{\rho_{0,c} = \frac{\Lambda c^2}{3H_0^2} \to \rho_{\Lambda}(t) \propto e^{\sqrt{\frac{\Lambda}{3}t}}$

Letâ€™s start with the first Friedmann equation (written in terms of the Hubble parameter now).

$$H^2(t) = \frac{8\piG}{3} \big ( \rho(t) - \frac{3k}{8\pi G a^2(t)} \big)$$

But $\rho(t) \gg \frac{3k}{8\pi G a^2(t)$ so we can consider that $H^2(t) = \frac{8\piG}{3} \rho(t)$ and we remember that $\Omega = \frac{\rho(t)}{\rho_c} = \frac{8 \pi G \rho(t)}{3 H^2_0}$.

We can rearrange $\Omega_M =  \frac{8 \pi G}{3 H^2_0} \rho_M(t) = \frac{\rho_M(t)}{\rho_{0,c} = \frac{\rho_M(t)}{\rho_M(t_0) \frac{\rho_M(t_0)}{\rho_{0,c} = a^{-3}(t)\Omega_{M,0} = \Omega_{M,0} a^{-3}(t)$.

Then, $\rho_M(t) = \frac{3 H_0^2}{8 \pi G}\Omega_{M,0} a^{-3}(t)$ and we can do the same for the other consituants : 

$\rho_R(t) = \frac{3 H_0^2}{8 \pi G}\Omega_{R,0} a^{-4}(t)$

$\rho_k(t) = \frac{3 H_0^2}{8 \pi G}\Omega_{k,0} a^{-2}(t)$

$\rho_{\Lambda}(t) = \frac{3 H_0^2}{8 \pi G}\Omega_{\Lambda}$

So, as $H^2(t) = \frac{8\piG}{3} \rho(t) \to H^2(t) = H_0^2\frac{8\piG}{3H_0^2} \big (\rho_M(t) + \rho_R(t) +  \rho_k(t) + \rho_{\Lambda}(t)$

$$H(t)^2 = H_0^2 \frac{1}{\rho_c} \big (\rho_M(t) + \rho_R(t) +  \rho_k(t) + \rho_{\Lambda}(t)$$

$$H(t)^2 = H_0^2 \frac{1}{\rho_c} \big (\Omega_{M,0} a^{-3}(t) + \Omega_{R,0} a^{-4}(t) +  \Omega_{k,0} a^{-2}(t) + \Omega_{\Lambda}$$

 $\textbf{III - Equations and numerical solving}$ 


